src/Computation/FixComp.v
@@ -574,6 +574,21 @@ Module LeastFixedPointFun.
     eapply (Is_GreatestFixedPoint fDef fDef_monotone).
   Qed.
 
+  (* [unroll_LeastFixedPoint'] is for unrolling one layer of *)
+  (* recursion in the conclusion about a Fixpoint computation. *)
+
+  Lemma unroll_LeastFixedPoint'
+        {fDom : list Type}
+        {fCod : Type}
+        (fDef : funType fDom fCod -> funType fDom fCod)
+        (fDef_monotone : forall rec rec',
+            refineFun rec rec'
+            -> refineFun (fDef rec) (fDef rec'))
+    : refineFun (LeastFixedPoint fDef) (fDef (LeastFixedPoint fDef)).
+  Proof.
+    eapply (Is_GreatestFixedPoint fDef fDef_monotone).
+  Qed.
+
   Lemma refine_LeastFixedPoint
         {fDom : list Type}
         {fCod : Type}
